pcuic/theories/Syntax/PCUICUnivSubst.v
@@ -8,11 +8,23 @@ Instance subst_instance_list A `{UnivSubst A} : UnivSubst (list A) :=
   fun u => List.map (subst_instance u).
 
 Lemma subst_instance_instance_length (u1 : Instance.t) u2 :
-  #|subst_instance u2 u1| = #|u1|.
+  Instance.eq_length (subst_instance u2 u1) u1.
 Proof.
-  unfold subst_instance.
-  now rewrite length_map.
+  unfold Instance.eq_length, subst_instance; split; now rewrite length_map.
 Qed.
+
+Lemma subst_instance_instance_length_univs (u1 : Instance.t) u2 :
+  #|Instance.universes (subst_instance u2 u1)| = #|Instance.universes u1|.
+Proof.
+  apply subst_instance_instance_length.
+Qed.
+
+Lemma subst_instance_instance_length_quals (u1 : Instance.t) u2 :
+  #|Instance.qualities (subst_instance u2 u1)| = #|Instance.qualities u1|.
+Proof.
+  apply subst_instance_instance_length.
+Qed.
+
 #[global]
 Hint Rewrite subst_instance_instance_length : len.
 
@@ -94,16 +106,25 @@ Proof.
       try solve [f_equal; eauto; repeat (rtoProp; solve_all); eauto with substu].
 Qed.
 
-Lemma subst_instance_closedu (u : Instance.t) (Hcl : closedu_instance 0 u) t :
-  closedu #|u| t -> closedu 0 (subst_instance u t).
+Lemma subst_instance_closedu (u : Instance.t) (Hcl : closed_instance 0 u) t :
+  closedu #|Instance.qualities u| t -> closedu #|Instance.universes u| t -> closedu 0 (subst_instance u t).
 Proof.
-  induction t in |- * using term_forall_list_ind; simpl; auto; intros H';
+  induction t in |- * using term_forall_list_ind; simpl; auto; intros ??;
     autorewrite with map;
     try f_equal; auto with substu;
       unfold test_def, test_predicate_ku, test_branch in *; simpl;
-      try solve [f_equal; eauto; repeat (rtoProp; solve_all); intuition auto with substu].
-  rewrite [#|subst_instance_instance _ _|]subst_instance_instance_length. solve_all.
-  eauto with substu.
+    try solve [f_equal; eauto; repeat (rtoProp; solve_all); intuition auto with substu].
+  
+  destruct p as [? []]; cbn in *; auto.
+  repeat rewrite andb_and in H0, H; destruct H as [[[Hql Hqf] Hqd] Hqt]; destruct H0 as [[[Hul Huf] Hud] Hut].
+  destruct X as [Xt [Xd Xv]]. repeat rewrite andb_and; repeat split.
+  - eauto with substu.
+  - apply All_forallb, All_map, In_All. intros t' H. eapply All_In in Xv; eauto.
+    elim Xv. intro. apply H0.
+    + eapply forallb_All, All_In in Hqf; eauto. elim Hqf. tauto.
+    + eapply forallb_All, All_In in Huf; eauto. elim Huf. tauto.
+  - apply Xd; auto.
+  - apply Xt; auto.
 Qed.
 
 Lemma rev_subst_instance {u Γ} :
