pcuic/theories/utils/PCUICAstUtils.v
@@ -29,10 +29,10 @@ Fixpoint string_of_term (t : term) :=
   | tLetIn na b t' t => "LetIn(" ^ string_of_aname na ^ "," ^ string_of_term b
                                  ^ "," ^ string_of_term t' ^ "," ^ string_of_term t ^ ")"
   | tApp f l => "App(" ^ string_of_term f ^ "," ^ string_of_term l ^ ")"
-  | tConst c u => "Const(" ^ string_of_kername c ^ "," ^ string_of_universe_instance u ^ ")"
-  | tInd i u => "Ind(" ^ string_of_inductive i ^ "," ^ string_of_universe_instance u ^ ")"
+  | tConst c u => "Const(" ^ string_of_kername c ^ "," ^ string_of_instance u ^ ")"
+  | tInd i u => "Ind(" ^ string_of_inductive i ^ "," ^ string_of_instance u ^ ")"
   | tConstruct i n u => "Construct(" ^ string_of_inductive i ^ "," ^ string_of_nat n ^ ","
-                                    ^ string_of_universe_instance u ^ ")"
+                                    ^ string_of_instance u ^ ")"
   | tCase ci p t brs =>
     "Case(" ^ string_of_case_info ci ^ "," ^ string_of_term t ^ ","
             ^ string_of_predicate string_of_term p ^ "," ^ string_of_list (string_of_branch string_of_term) brs ^ ")"
