template-rocq/theories/WfAst.v
@@ -133,9 +133,9 @@ Lemma term_wf_forall_list_ind Σ :
         P t -> forall t0 : term, P t0 -> forall t1 : term, P t1 -> P (tLetIn n t t0 t1)) ->
     (forall t : term, isApp t = false -> wf Σ t -> P t ->
                       forall l : list term, l <> nil -> All (wf Σ) l -> All P l -> P (tApp t l)) ->
-    (forall s (u : list Level.t), P (tConst s u)) ->
-    (forall (i : inductive) (u : list Level.t), P (tInd i u)) ->
-    (forall (i : inductive) (n : nat) (u : list Level.t),
+    (forall s (u : Instance.t), P (tConst s u)) ->
+    (forall (i : inductive) (u : Instance.t), P (tInd i u)) ->
+    (forall (i : inductive) (n : nat) (u : Instance.t),
       P (tConstruct i n u)) ->
     (forall (ci : case_info) (p : predicate term) mdecl idecl,
         declared_inductive Σ ci.(ci_ind) mdecl idecl ->
